state monad not depending on the definition of state

src/ParametricStateMonad.v
@@ -33,17 +33,72 @@ Instance state_Functor (s : Type)
   
 Next Obligation. apply state_functor_identity. Defined.
 
-Definition state_comp_apply {s} {a b} (f : state_comp s (a -> b)) (fs : state_comp s a)
+Definition state_comp_apply {s}{a b} (f : state_comp s (a -> b)) (fs : state_comp s a)
   : state_comp s b := 
   fun s => let (x, s'):= fs s in let (g, s''):= f s' in (g x, s'').
 
-Definition state_comp_pure {s}{a}(x:a): state_comp s a :=
+Definition state_comp_pure {s} {a}(x:a) : state_comp s a :=
 fun s => (x, s).
 
-Lemma state_applicative_identity {s}{a} (v : state_comp s a):
+Lemma state_comp_applicative_identity {s} {a}
+  (v : state_comp s  a):
   state_comp_apply (state_comp_pure id) v = v.
-Proof. unfold state_comp_apply. apply functional_extensionality. intros. 
+  Proof. unfold state_comp_apply. apply functional_extensionality. intros. 
 destruct (v x). unfold state_comp_pure. auto. Qed.
+
+Lemma state_comp_applicative_homomorphism {s} {a b} (v : a -> b) (x : a)
+  : state_comp_apply (state_comp_pure v) (state_comp_pure x) = state_comp_pure (s:=s) (v x).
+Proof. unfold state_comp_apply. apply functional_extensionality. intros. 
+unfold state_comp_pure. auto. Qed.
+
+Lemma state_comp_applicative_interchange {s}{a b}(u : state_comp s (a -> b)) (y : a)
+  : state_comp_apply u (state_comp_pure y) = state_comp_apply (state_comp_pure (fun z : a -> b => z y)) u.
+
+Proof. unfold state_comp_apply. apply functional_extensionality. intros. 
+unfold state_comp_pure. auto. Qed.
+
+#[program]
+Instance state_Applicative {s}
+  : Applicative (state_comp s) :=
+  { pure := @state_comp_pure s 
+  ; apply := @state_comp_apply s 
+  }.
+  
+Next Obligation. apply state_comp_applicative_identity. Defined.
+Next Obligation. unfold state_comp_apply, state_comp_pure.
+apply functional_extensionality. intros.  destruct (w x). destruct (v s0). 
+destruct (u s1). auto. Defined.
+Next Obligation. unfold state_comp_apply, state_comp_pure, state_comp_map.
+apply functional_extensionality. intros. destruct (x x0). auto. Defined.
+
+Definition state_comp_bind {s} {a b}
+  (r : state_comp s a) (f : a -> state_comp s b)
+  : state_comp s b :=
+  fun s => 
+              let (v, s') := r s in 
+              f v s'.
+
+Lemma state_bind_associativity {s} {a b c} 
+  (f : state_comp s a) (g : a -> state_comp s b) (h : b -> state_comp s c)
+  : state_comp_bind (state_comp_bind f g) h = 
+  state_comp_bind f (fun x : a => state_comp_bind (g x) h).
+Proof. unfold state_comp_bind. apply functional_extensionality. intros. 
+destruct (f x). destruct (g a0). trivial. Qed.
+
+#[program]
+Instance state_comp_Monad {s}
+  : Monad (state_comp s) :=
+  { bind := @state_comp_bind s
+  }.
+  
+Next Obligation. unfold state_comp_bind, state_comp_pure. 
+apply functional_extensionality. intros.
+destruct (x x0). trivial. Defined.
+Next Obligation. apply state_bind_associativity. Defined.
+Next Obligation. unfold state_comp_bind, state_comp_map, state_comp_pure.
+apply functional_extensionality. intros. destruct (x x0). trivial. Defined.
+
+
 
 
 
